@prefix : <https://w3id.org/un/ontology/undo/> .
@prefix dc: <http://purl.org/dc/elements/1.1/> .
@prefix dcterms: <http://purl.org/spar/dcterms/> .
@prefix dul: <http://www.ontologydesignpatterns.org/ont/dul/DUL.owl#> .
@prefix fabio: <http://purl.org/spar/fabio/> .
@prefix frbr: <http://purl.org/vocab/frbr/core#> .
@prefix lan: <http://id.loc.gov/vocabulary/iso639-1/> .
@prefix lkif-action: <http://www.estrellaproject.org/lkif-core/action.owl#> .
@prefix lkif-role: <http://www.estrellaproject.org/lkif-core/role.owl#> .
@prefix ns1: <http://purl.org/vocab/vann/> .
@prefix oa: <http://www.w3.org/ns/oa#> .
@prefix owl: <http://www.w3.org/2002/07/owl#> .
@prefix pro: <http://purl.org/spar/pro/> .
@prefix pso: <http://purl.org/spar/pso/> .
@prefix pwo: <http://purl.org/spar/pwo/> .
@prefix rdf: <http://www.w3.org/1999/02/22-rdf-syntax-ns#> .
@prefix rdfs: <http://www.w3.org/2000/01/rdf-schema#> .
@prefix skos: <http://www.w3.org/2004/02/skos/core#> .
@prefix ti: <http://www.ontologydesignpatterns.org/cp/owl/timeinterval.owl#> .
@prefix tvc: <http://www.essepuntato.it/2012/04/tvc/> .
@prefix xml: <http://www.w3.org/XML/1998/namespace> .
@prefix xsd: <http://www.w3.org/2001/XMLSchema#> .

lan:ar a owl:NamedIndividual,
        :Language ;
    rdfs:label "Arabic"@en ;
    dc:description "This entity representing the Arabic language has been originally defined in the Library of Congress concept scheme (skos:ConceptScheme) available at http://id.loc.gov/vocabulary/iso639-1, which maps all the two-letters codes for languages introduced in the specification ISO 639-1 as Linked Open Data."@en ;
    rdfs:comment "The Arabic is one of the languages used for publishing United Nations documents."@en ;
    rdfs:isDefinedBy <http://id.loc.gov/vocabulary/iso639-1> .

lan:en a owl:NamedIndividual,
        :Language ;
    rdfs:label "English"@en ;
    dc:description "This entity representing the English language has been originally defined in the Library of Congress concept scheme (skos:ConceptScheme) available at http://id.loc.gov/vocabulary/iso639-1, which maps all the two-letters codes for languages introduced in the specification ISO 639-1 as Linked Open Data."@en ;
    rdfs:comment "The English is one of the languages used for publishing United Nations documents."@en ;
    rdfs:isDefinedBy <http://id.loc.gov/vocabulary/iso639-1> .

lan:es a owl:NamedIndividual,
        :Language ;
    rdfs:label "Spanish"@en ;
    dc:description "This entity representing the Spanish language has been originally defined in the Library of Congress concept scheme (skos:ConceptScheme) available at http://id.loc.gov/vocabulary/iso639-1, which maps all the two-letters codes for languages introduced in the specification ISO 639-1 as Linked Open Data."@en ;
    rdfs:comment "The Spanish is one of the languages used for publishing United Nations documents."@en ;
    rdfs:isDefinedBy <http://id.loc.gov/vocabulary/iso639-1> .

lan:fr a owl:NamedIndividual,
        :Language ;
    rdfs:label "French"@en ;
    dc:description "This entity representing the French language has been originally defined in the Library of Congress concept scheme (skos:ConceptScheme) available at http://id.loc.gov/vocabulary/iso639-1, which maps all the two-letters codes for languages introduced in the specification ISO 639-1 as Linked Open Data."@en ;
    rdfs:comment "The French is one of the languages used for publishing United Nations documents."@en ;
    rdfs:isDefinedBy <http://id.loc.gov/vocabulary/iso639-1> .

lan:ru a owl:NamedIndividual,
        :Language ;
    rdfs:label "Russian"@en ;
    dc:description "This entity representing the Russian language has been originally defined in the Library of Congress concept scheme (skos:ConceptScheme) available at http://id.loc.gov/vocabulary/iso639-1, which maps all the two-letters codes for languages introduced in the specification ISO 639-1 as Linked Open Data."@en ;
    rdfs:comment "The Russian is one of the languages used for publishing United Nations documents."@en ;
    rdfs:isDefinedBy <http://id.loc.gov/vocabulary/iso639-1> .

lan:zh a owl:NamedIndividual,
        :Language ;
    rdfs:label "Chinese"@en ;
    dc:description "This entity representing the Chinise language has been originally defined in the Library of Congress concept scheme (skos:ConceptScheme) available at http://id.loc.gov/vocabulary/iso639-1, which maps all the two-letters codes for languages introduced in the specification ISO 639-1 as Linked Open Data."@en ;
    rdfs:comment "The Chinese is one of the languages used for publishing United Nations documents."@en ;
    rdfs:isDefinedBy <http://id.loc.gov/vocabulary/iso639-1> .

frbr:transformation a owl:ObjectProperty ;
    rdfs:isDefinedBy <http://purl.org/vocab/frbr/core> .

owl:Thing a owl:Class .

<https://w3id.org/akn/ontology/allot/Organization> a owl:Class ;
    rdfs:isDefinedBy <https://w3id.org/akn/ontology/allot> ;
    rdfs:subClassOf lkif-action:Organisation,
        <http://xmlns.com/foaf/0.1/Organization>,
        :Agent .

<https://w3id.org/akn/ontology/allot/Person> rdfs:isDefinedBy <https://w3id.org/akn/ontology/allot> ;
    rdfs:subClassOf lkif-action:Person,
        <http://xmlns.com/foaf/0.1/Person>,
        :Agent .

<https://w3id.org/akn/ontology/allot/Role> a owl:Class ;
    rdfs:isDefinedBy <https://w3id.org/akn/ontology/allot> ;
    rdfs:subClassOf pro:Role,
        lkif-role:Role,
        :Value .

<https://w3id.org/akn/ontology/allot/hasEmbodiment> rdfs:subPropertyOf frbr:embodiment .

<https://w3id.org/akn/ontology/allot/hasExemplar> rdfs:subPropertyOf frbr:exemplar .

<https://w3id.org/akn/ontology/allot/mentions> a owl:ObjectProperty .

:Address a owl:Class ;
    rdfs:label "address"@en ;
    rdfs:comment "A document exemplifying keynote speeches and opening addresses and messages."@en ;
    rdfs:isDefinedBy <https://w3id.org/un/ontology/undo> ;
    rdfs:subClassOf :Communication .

:AdministrativeCircular a owl:Class ;
    rdfs:label "administrative circular"@en ;
    rdfs:comment "A document containing general information of administrative nature as well as clarifications of established rules, policies and procedures."@en ;
    rdfs:isDefinedBy <https://w3id.org/un/ontology/undo> ;
    rdfs:subClassOf :AdministrativeIssuance .

:AdministrativeInstruction a owl:Class ;
    rdfs:label "administrative instruction"@en ;
    rdfs:comment "A document that prescribes instructions and procedures for the implementation of rules and regulations, as well as formally communicate decisions on, for example, appointment, promotion, transfer and change of duty station."@en ;
    rdfs:isDefinedBy <https://w3id.org/un/ontology/undo> ;
    rdfs:subClassOf :AdministrativeIssuance .

:AdvisoryOpinion a owl:Class ;
    rdfs:label "advisory opinion"@en ;
    rdfs:comment "A document introducing an opinion rendered by a court or adjudicating body upon request."@en ;
    rdfs:isDefinedBy <https://w3id.org/un/ontology/undo> ;
    rdfs:subClassOf :CourtDecision .

:AgendaListing a owl:Class ;
    rdfs:label "agenda listing"@en ;
    rdfs:comment "A document listing agenda items to be considered at a specific meeting/s or session/s. It may report time, location, etc."@en ;
    rdfs:isDefinedBy <https://w3id.org/un/ontology/undo> ;
    rdfs:subClassOf :MeetingAgenda .

:Amendment a owl:Class ;
    rdfs:label "amendment"@en ;
    rdfs:comment "A document that provides modifications to other normative documents. The modifications could appear in different structured texts like normative and deliberative documents, debate records, etc."@en ;
    rdfs:isDefinedBy <https://w3id.org/un/ontology/undo> ;
    rdfs:subClassOf :ModificatoryInstruction .

:AmendmentList a owl:Class ;
    rdfs:label "amendment list"@en ;
    rdfs:comment "A document listing proposals for modifications submitted to official deliberative bodies for discussion. It provides modifications to other normative documents."@en ;
    rdfs:isDefinedBy <https://w3id.org/un/ontology/undo> ;
    rdfs:subClassOf :ModificatoryInstruction .

:AnnotatedAgenda a owl:Class ;
    rdfs:label "annotated agenda"@en ;
    rdfs:comment "An agenda with a brief description of agenda items, citation of related documents as well as information and other announcements."@en ;
    rdfs:isDefinedBy <https://w3id.org/un/ontology/undo> ;
    rdfs:subClassOf :MeetingAgenda .

:Annotation a owl:Class ;
    rdfs:label "annotation"@en ;
    rdfs:comment "A mechanism that allows someone to link a specific entity (e.g. a relation) to a target document (or its parts), with the intent of specifying from where that entity has been actually derived from."@en ;
    rdfs:isDefinedBy <https://w3id.org/un/ontology/undo> ;
    rdfs:subClassOf [ a owl:Restriction ;
            owl:allValuesFrom <https://w3id.org/akn/ontology/allot/Reference> ;
            owl:onProperty oa:hasBody ],
        [ a owl:Restriction ;
            owl:allValuesFrom [ a owl:Class ;
                    owl:unionOf ( <https://w3id.org/akn/ontology/allot/FRBRExpression> <https://w3id.org/akn/ontology/allot/FRBRItem> <https://w3id.org/akn/ontology/allot/FRBRManifestation> <https://w3id.org/akn/ontology/allot/FRBRWork> ) ] ;
            owl:onProperty oa:hasTarget ],
        oa:Annotation,
        <https://w3id.org/akn/ontology/allot/Concept> .

:Bulletin a owl:Class ;
    rdfs:label "bulletin"@en ;
    rdfs:comment "A document containing information not requiring any action by the addressees."@en ;
    rdfs:isDefinedBy <https://w3id.org/un/ontology/undo> ;
    rdfs:subClassOf :Communication .

:Charter a owl:Class ;
    rdfs:label "charter"@en ;
    rdfs:comment "Foundational treaty outlining the conditions under which a body is organised, and defining its rights and privileges."@en ;
    rdfs:isDefinedBy <https://w3id.org/un/ontology/undo> ;
    rdfs:subClassOf :NormativeDocument .

:Circular a owl:Class ;
    rdfs:label "circular"@en ;
    rdfs:comment "A document containing specialized information of specific interests."@en ;
    rdfs:isDefinedBy <https://w3id.org/un/ontology/undo> ;
    rdfs:subClassOf :Communication .

:CodeOfConduct a owl:Class ;
    rdfs:label "code of conduct"@en ;
    rdfs:comment "A document listing rules outlining the responsibilities of, or proper practices for, individuals, parties, organizations, or countries on specific issues."@en ;
    rdfs:isDefinedBy <https://w3id.org/un/ontology/undo> ;
    rdfs:subClassOf :NormativeDocument .

:CodeOfPractice a owl:Class ;
    rdfs:label "code of practice"@en ;
    rdfs:comment "A document that defines correct procedures on how to implement principles and/or standards."@en ;
    rdfs:isDefinedBy <https://w3id.org/un/ontology/undo> ;
    rdfs:subClassOf :NormativeDocument .

:Collection a owl:Class ;
    rdfs:label "collection"@en ;
    rdfs:comment "A collection of individual autonomous documents."@en ;
    rdfs:isDefinedBy <https://w3id.org/un/ontology/undo> ;
    rdfs:subClassOf :Publication .

:ConferenceReport a owl:Class ;
    rdfs:label "conference report"@en ;
    rdfs:comment "A document summarising discussions held during a conference. It may also contain full text of resolutions or decisions, either proposed or adopted; recommended actions to be taken by other organs, etc., in the body of the document or as annexes."@en ;
    rdfs:isDefinedBy <https://w3id.org/un/ontology/undo> ;
    rdfs:subClassOf :MeetingReport .

:Constitution a owl:Class ;
    rdfs:label "constitution"@en ;
    rdfs:comment "A document describing a set of fundamental principles or established precedents according to which a body is acknowledged to be governed."@en ;
    rdfs:isDefinedBy <https://w3id.org/un/ontology/undo> ;
    rdfs:subClassOf :NormativeDocument .

:Convention a owl:Class ;
    rdfs:label "convention"@en ;
    rdfs:comment "Mandatory regulations subject to ratification. Instruments usually negotiated under the auspices of an international organization."@en ;
    rdfs:isDefinedBy <https://w3id.org/un/ontology/undo> ;
    rdfs:subClassOf :NormativeDocument .

:CouncilReport a owl:Class ;
    rdfs:label "council report"@en ;
    rdfs:comment "A document summarising discussions held during a council. It may also contain full text of resolutions or decisions, either proposed or adopted; recommended actions to be taken by other organs, etc., in the body of the document or as annexes."@en ;
    rdfs:isDefinedBy <https://w3id.org/un/ontology/undo> ;
    rdfs:subClassOf :MeetingReport .

:Decision a owl:Class ;
    rdfs:label "decision"@en ;
    rdfs:comment "A document describing a formal action regarding administrative and procedural matters of principal or subsidiary organ or other empowered bodies. This kind of documents is sometimes also used to record the adoption of a text representing the consensus of the members of a given organ."@en ;
    rdfs:isDefinedBy <https://w3id.org/un/ontology/undo> ;
    rdfs:subClassOf :DeliberativeDocument .

:Judgment a owl:Class ;
    rdfs:label "judgement"@en ;
    rdfs:comment "A document formalising a decision or specific determination following a legal proceeding. Its structures are highly formalised."@en ;
    rdfs:isDefinedBy <https://w3id.org/un/ontology/undo> ;
    rdfs:subClassOf :CourtDecision .

:LegalSource a owl:Class ;
    rdfs:label "legal source"@en ;
    rdfs:comment "A source of one or more legal norms formulated in any format and endorsed by an authority."@en ;
    rdfs:isDefinedBy <https://w3id.org/un/ontology/undo> ;
    rdfs:subClassOf <https://w3id.org/akn/ontology/allot/FRBRWork> .

:MeetingMinute a owl:Class ;
    rdfs:label "meeting minute"@en ;
    rdfs:comment "A document providing a third-person accounts of meetings."@en ;
    rdfs:isDefinedBy <https://w3id.org/un/ontology/undo> ;
    rdfs:subClassOf :MeetingReport .

:MeetingRecord a owl:Class ;
    rdfs:label "meeting record"@en ;
    rdfs:comment "Documents containing full first-person records of a meeting (verbatim). Their structure reflects the different section of the debates and/or alternation of questions and answers that take place during meetings discussions."@en ;
    rdfs:isDefinedBy <https://w3id.org/un/ontology/undo> ;
    rdfs:subClassOf :Document .

:Memoranda a owl:Class ;
    rdfs:label "memoranda"@en ;
    rdfs:comment "An official written communication issued to disseminate information."@en ;
    rdfs:isDefinedBy <https://w3id.org/un/ontology/undo> ;
    rdfs:subClassOf :Communication .

:Note a owl:Class ;
    rdfs:label "note"@en ;
    rdfs:comment "A written communication to transmit comments or reports."@en ;
    rdfs:isDefinedBy <https://w3id.org/un/ontology/undo> ;
    rdfs:subClassOf :Communication .

:OfficialCompilation a owl:Class ;
    rdfs:label "official compilation"@en ;
    rdfs:comment "An authoritative compilation of official documents."@en ;
    rdfs:isDefinedBy <https://w3id.org/un/ontology/undo> ;
    rdfs:subClassOf :Publication .

:OfficialLetter a owl:Class ;
    rdfs:label "official letter"@en ;
    rdfs:comment "Official written correspondence; communications or notes verbale concerning issues under the authority of the organisation to provide information, requiring specific action by the addressees or stating a position."@en ;
    rdfs:isDefinedBy <https://w3id.org/un/ontology/undo> ;
    rdfs:subClassOf :Communication .

:OfficialStatement a owl:Class ;
    rdfs:label "official statement"@en ;
    rdfs:comment "A document introducing a pronunciation of officers in their official capacity."@en ;
    rdfs:isDefinedBy <https://w3id.org/un/ontology/undo> ;
    rdfs:subClassOf :Communication .

:Policy a owl:Class ;
    rdfs:label "policy"@en ;
    rdfs:comment "A document introducing general course or principle of action adopted or proposed by the official authorities or bodies."@en ;
    rdfs:isDefinedBy <https://w3id.org/un/ontology/undo> ;
    rdfs:subClassOf :Paper .

:PositionPaper a owl:Class ;
    rdfs:label "position paper"@en ;
    rdfs:comment "An essay detailing facts and opinions regarding specific issues."@en ;
    rdfs:isDefinedBy <https://w3id.org/un/ontology/undo> ;
    rdfs:subClassOf :Paper .

:PressRelease a owl:Class ;
    rdfs:label "press release"@en ;
    rdfs:comment "A written communication to the public that serves information purposes only. It is not considered an official document."@en ;
    rdfs:isDefinedBy <https://w3id.org/un/ontology/undo> ;
    rdfs:subClassOf :Communication .

:ProgressReport a owl:Class ;
    rdfs:label "progress report"@en ;
    rdfs:comment "A document assessing projects or processes."@en ;
    rdfs:isDefinedBy <https://w3id.org/un/ontology/undo> ;
    rdfs:subClassOf :Paper .

:Protocol a owl:Class ;
    rdfs:label "protocol"@en ;
    rdfs:comment "International agreement that supplements a previous treaty or international agreement."@en ;
    rdfs:isDefinedBy <https://w3id.org/un/ontology/undo> ;
    rdfs:subClassOf :NormativeDocument .

:Recommendation a owl:Class ;
    rdfs:label "recommendation"@en ;
    rdfs:comment "A document that provides guidance and may create reporting obligations for parties."@en ;
    rdfs:isDefinedBy <https://w3id.org/un/ontology/undo> ;
    rdfs:subClassOf :NormativeDocument .

:Regulation a owl:Class ;
    rdfs:label "regulation"@en ;
    rdfs:comment "A set guides to enforce a statutory instrument or regulate activities."@en ;
    rdfs:isDefinedBy <https://w3id.org/un/ontology/undo> ;
    rdfs:subClassOf :NormativeDocument .

:Resolution a owl:Class ;
    rdfs:label "resolution"@en ;
    rdfs:comment "A particular kind of document that contains a formal expression of the will of a principal or subsidiary organ or other empowered bodies."@en ;
    rdfs:isDefinedBy <https://w3id.org/un/ontology/undo> ;
    rdfs:subClassOf :DeliberativeDocument .

:Rules a owl:Class ;
    rdfs:label "rules"@en ;
    rdfs:comment "A document prescribing principles governing conduct or procedure within a particular area of activity."@en ;
    rdfs:isDefinedBy <https://w3id.org/un/ontology/undo> ;
    rdfs:subClassOf :NormativeDocument .

:RulesOfProcedure a owl:Class ;
    rdfs:label "rules of procedure"@en ;
    rdfs:comment "A document that prescribes guides for conduct or actions, such as rules for conducting business within a body, as well as for the financial administration of organizations and their members."@en ;
    rdfs:isDefinedBy <https://w3id.org/un/ontology/undo> ;
    rdfs:subClassOf :NormativeDocument .

:Standard a owl:Class ;
    rdfs:label "standard"@en ;
    rdfs:comment "A document introducing a set of guides established by consensus outlining the responsibilities of, or proper practices for, individuals, parties, organizations or countries on specific issues."@en ;
    rdfs:isDefinedBy <https://w3id.org/un/ontology/undo> ;
    rdfs:subClassOf :NormativeDocument .

:Status a owl:Class ;
    rdfs:label "status"@en ;
    rdfs:comment "A value identifying the status of a document (e.g. in drafting, under revision, published)."@en ;
    rdfs:isDefinedBy <https://w3id.org/un/ontology/undo> ;
    rdfs:subClassOf pso:Status,
        :Value .

:Treaty a owl:Class ;
    rdfs:label "treaty"@en ;
    rdfs:comment "An international agreement concluded between States, and bilateral or multilateral agreements governed by international law to which international organizations are parties."@en ;
    rdfs:isDefinedBy <https://w3id.org/un/ontology/undo> ;
    rdfs:subClassOf :NormativeDocument .

:ValueInTimeAndContext a owl:Class ;
    rdfs:label "value in time and context"@en ;
    dc:description """This class is based on a particular ontology pattern called Time-indexed Value in Context (http://www.essepuntato.it/2012/04/tvc). It has been used by several ontologies for describing values that can be assigned/held by an entity at different times and according to different contexts. Notable ontologies that are using it are the Publishing Roles Ontology (PRO, http://purl.org/spar/pro) and the Publishing Status Ontology (PSO, http://purl.org/spar/pso).

More information are available at the following paper:

Peroni, S., Shotton, D., Vitali, F. (2012). Scholarly publishing and the Linked Data: describing roles, statuses, temporal and contextual extents. In Sack, H., Pellegrini, T. (Eds.), Proceedings of the 8th International Conference on Semantic Systems (i-Semantics 2012): 9-16. New York, New York, USA: ACM. DOI: http://dx.doi.org/10.1145/2362499.2362502 (Open Access version available at http://speroni.web.cs.unibo.it/publications/peroni-2012-scholarly-publishing-linked.pdf)"""@en ;
    rdfs:comment "The situation that involves an entity (with the object property tvc:hasValue) having a particular value (tvc:withValue) associated during a certain time interval (tvc:atTime) and within a specific context (tvc:withinContext)."@en ;
    rdfs:isDefinedBy <https://w3id.org/un/ontology/undo> ;
    rdfs:subClassOf [ a owl:Restriction ;
            owl:allValuesFrom :Interval ;
            owl:onProperty tvc:atTime ],
        [ a owl:Restriction ;
            owl:allValuesFrom :Value ;
            owl:onProperty tvc:withValue ],
        [ a owl:Restriction ;
            owl:allValuesFrom <https://w3id.org/akn/ontology/allot/Reference> ;
            owl:onProperty tvc:withinContext ],
        [ a owl:Restriction ;
            owl:allValuesFrom <https://w3id.org/akn/ontology/allot/Reference> ;
            owl:onProperty [ owl:inverseOf tvc:hasValue ] ],
        tvc:ValueInTime,
        <https://w3id.org/akn/ontology/allot/Concept> .

:WorkflowExecution a owl:Class ;
    rdfs:label "workflow execution"@en ;
    rdfs:comment "A collection of actions that address all the step defined in a workflow."@en ;
    rdfs:isDefinedBy <https://w3id.org/un/ontology/undo> ;
    rdfs:subClassOf [ a owl:Restriction ;
            owl:allValuesFrom :Workflow ;
            owl:onProperty pwo:executes ],
        [ a owl:Restriction ;
            owl:allValuesFrom :Action ;
            owl:onProperty pwo:involvesAction ],
        pwo:WorkflowExecution,
        <https://w3id.org/akn/ontology/allot/Concept> .

:hasLifecycleRevision a owl:ObjectProperty ;
    rdfs:label "has lifecycle revision"@en ;
    rdfs:comment "It links a document version with another altered or updated version of it as consequence of an event of a lifecycle."@en ;
    rdfs:domain :DocumentVersion ;
    rdfs:isDefinedBy <https://w3id.org/un/ontology/undo> ;
    rdfs:range [ a owl:Class ;
            owl:intersectionOf ( :DocumentVersion [ a owl:Restriction ;
                        owl:onProperty [ owl:inverseOf pwo:produces ] ;
                        owl:someValuesFrom [ a owl:Class ;
                                owl:intersectionOf ( <https://w3id.org/akn/ontology/allot/Event> [ a owl:Restriction ;
                                            owl:onProperty [ owl:inverseOf :includesEvent ] ;
                                            owl:someValuesFrom :Lifecycle ] ) ] ] ) ] ;
    rdfs:subPropertyOf frbr:revision,
        <https://w3id.org/akn/ontology/allot/hasRelatedReference> .

:hasRelatedConcept a owl:ObjectProperty ;
    rdfs:label "has related concept"@en ;
    rdfs:comment "A concept that is related somehow to a term (e.g. because it represents the meaning of a particular term)."@en ;
    rdfs:domain <https://w3id.org/akn/ontology/allot/Term> ;
    rdfs:isDefinedBy <https://w3id.org/un/ontology/undo> ;
    rdfs:range <https://w3id.org/akn/ontology/allot/Concept> ;
    rdfs:subPropertyOf <https://w3id.org/akn/ontology/allot/hasRelatedReference> .

:hasStepType a owl:ObjectProperty ;
    rdfs:domain :Step ;
    rdfs:isDefinedBy <https://w3id.org/un/ontology/undo> ;
    rdfs:range :StepType ;
    rdfs:subPropertyOf <https://w3id.org/akn/ontology/allot/hasRelatedReference> .

<http://purl.org/dc/terms/LinguisticSystem> a owl:Class ;
    rdfs:isDefinedBy <http://purl.org/dc/terms/> .

fabio:Expression a owl:Class ;
    rdfs:isDefinedBy <http://purl.org/spar/fabio> .

fabio:Item a owl:Class ;
    rdfs:isDefinedBy <http://purl.org/spar/fabio> .

fabio:Manifestation a owl:Class ;
    rdfs:isDefinedBy <http://purl.org/spar/fabio> .

fabio:Work a owl:Class ;
    rdfs:isDefinedBy <http://purl.org/spar/fabio> .

pro:Role a owl:Class ;
    rdfs:isDefinedBy <http://purl.org/spar/pro> .

pso:Status a owl:Class ;
    rdfs:isDefinedBy <http://purl.org/spar/pso> .

frbr:Expression a owl:Class .

frbr:Item a owl:Class .

frbr:Manifestation a owl:Class .

frbr:Work a owl:Class .

frbr:embodiment a owl:ObjectProperty ;
    rdfs:isDefinedBy <http://purl.org/vocab/frbr/core> .

frbr:exemplar a owl:ObjectProperty ;
    rdfs:isDefinedBy <http://purl.org/vocab/frbr/core> .

frbr:realization a owl:ObjectProperty ;
    rdfs:isDefinedBy <http://purl.org/vocab/frbr/core> .

frbr:revision a owl:ObjectProperty ;
    rdfs:isDefinedBy <http://purl.org/vocab/frbr/core> .

tvc:ValueInTime a owl:Class ;
    rdfs:isDefinedBy <http://www.essepuntato.it/2012/04/tvc> .

tvc:atTime a owl:ObjectProperty ;
    rdfs:isDefinedBy <http://www.essepuntato.it/2012/04/tvc> .

tvc:hasValue a owl:ObjectProperty ;
    rdfs:isDefinedBy <http://www.essepuntato.it/2012/04/tvc> .

tvc:withValue a owl:ObjectProperty ;
    rdfs:isDefinedBy <http://www.essepuntato.it/2012/04/tvc> .

tvc:withinContext a owl:ObjectProperty ;
    rdfs:isDefinedBy <http://www.essepuntato.it/2012/04/tvc> .

lkif-action:Agent a owl:Class ;
    rdfs:isDefinedBy <http://www.estrellaproject.org/lkif-core/action.owl> .

lkif-action:Organisation a owl:Class ;
    rdfs:isDefinedBy <http://www.estrellaproject.org/lkif-core/action.owl> .

lkif-action:Person a owl:Class ;
    rdfs:isDefinedBy <http://www.estrellaproject.org/lkif-core/action.owl> .

lkif-role:Role a owl:Class ;
    rdfs:isDefinedBy <http://www.estrellaproject.org/lkif-core/role.owl> .

ti:TimeInterval a owl:Class ;
    rdfs:isDefinedBy <http://www.ontologydesignpatterns.org/cp/owl/timeinterval.owl> .

ti:hasIntervalEndDate a owl:DatatypeProperty ;
    rdfs:comment <http://www.ontologydesignpatterns.org/cp/owl/timeinterval.owl> .

ti:hasIntervalStartDate a owl:DatatypeProperty ;
    rdfs:comment <http://www.ontologydesignpatterns.org/cp/owl/timeinterval.owl> .

oa:hasBody a owl:ObjectProperty ;
    rdfs:isDefinedBy oa: .

oa:hasTarget a owl:ObjectProperty ;
    rdfs:isDefinedBy oa: .

<http://xmlns.com/foaf/0.1/Agent> a owl:Class ;
    rdfs:isDefinedBy <http://xmlns.com/foaf/0.1/> .

<http://xmlns.com/foaf/0.1/Organization> a owl:Class ;
    rdfs:isDefinedBy <http://xmlns.com/foaf/0.1/> .

<http://xmlns.com/foaf/0.1/Person> a owl:Class ;
    rdfs:isDefinedBy <http://xmlns.com/foaf/0.1/> .

<https://w3id.org/akn/ontology/allot/FRBRItem> rdfs:isDefinedBy <https://w3id.org/akn/ontology/allot> ;
    rdfs:subClassOf fabio:Item,
        frbr:Item .

<https://w3id.org/akn/ontology/allot/FRBRManifestation> rdfs:isDefinedBy <https://w3id.org/akn/ontology/allot> ;
    rdfs:subClassOf fabio:Manifestation,
        frbr:Manifestation .

<https://w3id.org/akn/ontology/allot/Term> a owl:Class ;
    rdfs:isDefinedBy <https://w3id.org/akn/ontology/allot> .

:StepType a owl:Class ;
    rdfs:label "step type"@en ;
    rdfs:comment "The class of all the types for categorising the steps in workflow descriptions."@en ;
    rdfs:isDefinedBy <https://w3id.org/un/ontology/undo> ;
    rdfs:subClassOf <https://w3id.org/akn/ontology/allot/Concept> .

:Workflow a owl:Class ;
    rdfs:label "workflow"@en ;
    rdfs:comment "A description of a sequence of connected steps, representing a sequence of publishing operations undertaken by agents."@en ;
    rdfs:isDefinedBy <https://w3id.org/un/ontology/undo> ;
    rdfs:subClassOf [ a owl:Restriction ;
            owl:allValuesFrom :Step ;
            owl:onProperty pwo:hasStep ],
        pwo:Workflow,
        <https://w3id.org/akn/ontology/allot/Concept> .

:hasProponent a owl:ObjectProperty ;
    rdfs:label "has proponent"@en ;
    rdfs:comment "The proponent entity of a relation."@en ;
    rdfs:domain :Relation ;
    rdfs:isDefinedBy <https://w3id.org/un/ontology/undo> ;
    rdfs:range <https://w3id.org/akn/ontology/allot/Reference> ;
    rdfs:subPropertyOf <https://w3id.org/akn/ontology/allot/hasRelatedReference> .

:hasReceiver a owl:ObjectProperty ;
    rdfs:label "has receiver"@en ;
    rdfs:comment "The receiver entity of a relation."@en ;
    rdfs:domain :Relation ;
    rdfs:isDefinedBy <https://w3id.org/un/ontology/undo> ;
    rdfs:range <https://w3id.org/akn/ontology/allot/Reference> ;
    rdfs:subPropertyOf <https://w3id.org/akn/ontology/allot/hasRelatedReference> .

:hasSemantics a owl:ObjectProperty ;
    rdfs:label "has semantics"@en ;
    rdfs:comment "The semantics of a relation."@en ;
    rdfs:domain :Relation ;
    rdfs:isDefinedBy <https://w3id.org/un/ontology/undo> ;
    rdfs:range <https://w3id.org/akn/ontology/allot/Concept> ;
    rdfs:subPropertyOf <https://w3id.org/akn/ontology/allot/hasRelatedReference> .

<http://purl.org/dc/terms/language> a owl:ObjectProperty ;
    rdfs:label "has language"@en ;
    rdfs:comment "This property enables one to specify the language associated to a particular document version."@en ;
    rdfs:isDefinedBy <http://purl.org/dc/terms> .

<https://w3id.org/akn/ontology/allot/FRBRExpression> rdfs:isDefinedBy <https://w3id.org/akn/ontology/allot> ;
    rdfs:subClassOf [ a owl:Restriction ;
            owl:onClass :Language ;
            owl:onProperty <http://purl.org/dc/terms/language> ;
            owl:qualifiedCardinality "1"^^xsd:nonNegativeInteger ],
        fabio:Expression,
        frbr:Expression .

<https://w3id.org/akn/ontology/allot/hasRealization> a owl:ObjectProperty ;
    rdfs:subPropertyOf frbr:realization .

:Action a owl:Class ;
    rdfs:label "action"@en ;
    rdfs:comment "An event with at least one agent that is participant in it and that is linked to a workflow execution and to a step of a workflow description."@en ;
    rdfs:isDefinedBy <https://w3id.org/un/ontology/undo> ;
    rdfs:subClassOf [ a owl:Restriction ;
            owl:allValuesFrom :Interval ;
            owl:onProperty pwo:happened ],
        [ a owl:Restriction ;
            owl:allValuesFrom <https://w3id.org/akn/ontology/allot/Reference> ;
            owl:onProperty <http://www.ontologydesignpatterns.org/cp/owl/participation.owl#hasParticipant> ],
        [ a owl:Restriction ;
            owl:allValuesFrom :Step ;
            owl:onProperty <http://www.ontologydesignpatterns.org/cp/owl/taskexecution.owl#executesTask> ],
        pwo:Action,
        <https://w3id.org/akn/ontology/allot/Event> .

:AdministrativeIssuance a owl:Class ;
    rdfs:label "administrative issuance"@en ;
    rdfs:comment "Document concerning administrative instructions and circulars. Their structures vary widely across organizations and traditions but may have the format of a formal communication with a title and content in unnumbered or numbered paragraphs or be divided into sections."@en ;
    rdfs:isDefinedBy <https://w3id.org/un/ontology/undo> ;
    rdfs:subClassOf :Document .

:Agent a owl:Class ;
    rdfs:label "agent"@en ;
    rdfs:comment "An actor (e.g. a person, an organisation) that can perform some actions."@en ;
    rdfs:isDefinedBy <https://w3id.org/un/ontology/undo> ;
    rdfs:subClassOf lkif-action:Agent,
        dul:Agent,
        <http://xmlns.com/foaf/0.1/Agent>,
        <https://w3id.org/akn/ontology/allot/Reference> .

:CourtDecision a owl:Class ;
    rdfs:label "court decision"@en ;
    rdfs:comment "A document introducing a court of law or adjudicating authority formal decision or specific determination following a legal proceedings. The typical narrative of judgments is often divided in background, introduction, motivation and decision."@en ;
    rdfs:isDefinedBy <https://w3id.org/un/ontology/undo> ;
    rdfs:subClassOf :Document .

:DeliberativeDocument a owl:Class ;
    rdfs:label "deliberative document"@en ;
    rdfs:comment "Formal expressions of the opinion or will of a principal or subsidiary organ or other empowered bodies. Usually they are open structure documents, sometimes articulated in hierarchical structures in which the text is subdivided into higher and lower subdivisions, generally including a preamble and operative paragraphs."@en ;
    rdfs:isDefinedBy <https://w3id.org/un/ontology/undo> ;
    rdfs:subClassOf :Document .

:Lifecycle a owl:Class ;
    rdfs:label "lifecycle"@en ;
    rdfs:comment "A collection of events that a document has undergone, which also links to other documents that have caused these events."@en ;
    rdfs:isDefinedBy <https://w3id.org/un/ontology/undo> ;
    rdfs:subClassOf [ a owl:Restriction ;
            owl:allValuesFrom [ a owl:Class ;
                    owl:intersectionOf ( <https://w3id.org/akn/ontology/allot/Event> [ a owl:Restriction ;
                                owl:onProperty <http://www.ontologydesignpatterns.org/cp/owl/participation.owl#hasParticipant> ;
                                owl:someValuesFrom frbr:Endeavour ] [ a owl:Restriction ;
                                owl:allValuesFrom :Interval ;
                                owl:onProperty pwo:happened ] ) ] ;
            owl:onProperty :includesEvent ],
        <https://w3id.org/akn/ontology/allot/Concept> .

:MeetingAgenda a owl:Class ;
    rdfs:label "meeting agenda"@en ;
    rdfs:comment "Documents listing agenda items of a meeting or a series of meetings, at times with brief description of agenda items, citation of related documents, and other announcements, such as consultations, informal meetings or side events, as well as summaries of the previous day's meetings. Their structures vary widely across organizations and traditions."@en ;
    rdfs:isDefinedBy <https://w3id.org/un/ontology/undo> ;
    rdfs:subClassOf :Document .

:ModificatoryInstruction a owl:Class ;
    rdfs:label "modificatory instruction"@en ;
    rdfs:comment "A document containing formal proposals for modifications, as single instruction or as a collection of instructions, of previously issued documents issued by the same body that approved the original document. Its structures vary widely across organizations and traditions."@en ;
    rdfs:isDefinedBy <https://w3id.org/un/ontology/undo> ;
    rdfs:subClassOf :Document .

:Publication a owl:Class ;
    rdfs:label "publication"@en ;
    rdfs:comment "The documentary output of the process meant to share information in any form or medium."@en ;
    rdfs:isDefinedBy <https://w3id.org/un/ontology/undo> ;
    rdfs:subClassOf :Document .

:includesEvent a owl:ObjectProperty ;
    rdfs:label "includes event"@en ;
    rdfs:comment "It enables the specification of the events included in a document lifecycle."@en ;
    rdfs:domain :Lifecycle ;
    rdfs:isDefinedBy <https://w3id.org/un/ontology/undo> ;
    rdfs:range <https://w3id.org/akn/ontology/allot/Event> ;
    rdfs:subPropertyOf <https://w3id.org/akn/ontology/allot/hasRelatedReference> .

<https://w3id.org/akn/ontology/allot/FRBRWork> rdfs:isDefinedBy <https://w3id.org/akn/ontology/allot> ;
    rdfs:subClassOf fabio:Work,
        frbr:Work .

:DocumentVersion a owl:Class ;
    rdfs:label "document version"@en ;
    rdfs:comment "A particular version of a document written according to a certain language."@en ;
    rdfs:isDefinedBy <https://w3id.org/un/ontology/undo> ;
    rdfs:subClassOf [ a owl:Restriction ;
            owl:allValuesFrom :Document ;
            owl:onProperty [ owl:inverseOf <https://w3id.org/akn/ontology/allot/hasRealization> ] ],
        [ a owl:Restriction ;
            owl:onClass :Language ;
            owl:onProperty <http://purl.org/dc/terms/language> ;
            owl:qualifiedCardinality "1"^^xsd:nonNegativeInteger ],
        <https://w3id.org/akn/ontology/allot/FRBRExpression> .

:Interval a owl:Class ;
    rdfs:label "interval"@en ;
    rdfs:comment "A particular time period characterised by a starting date (specified by means of the property ti:hasIntervalStartDate) and an ending date (specified by means of the property ti:hasIntervalEndDate)."@en ;
    rdfs:isDefinedBy <https://w3id.org/un/ontology/undo> ;
    rdfs:subClassOf [ a owl:Restriction ;
            owl:allValuesFrom xsd:dateTime ;
            owl:onProperty ti:hasIntervalEndDate ],
        [ a owl:Restriction ;
            owl:allValuesFrom xsd:dateTime ;
            owl:onProperty ti:hasIntervalStartDate ],
        <http://purl.obolibrary.org/obo/BFO_0000038>,
        ti:TimeInterval,
        dul:TimeInterval,
        <https://w3id.org/akn/ontology/allot/Reference> .

:MeetingReport a owl:Class ;
    rdfs:label "meeting report"@en ;
    rdfs:comment "Documents containing summarized accounts of meetings. Their structures vary widely across organizations and traditions."@en ;
    rdfs:isDefinedBy <https://w3id.org/un/ontology/undo> ;
    rdfs:subClassOf :Document .

:Paper a owl:Class ;
    rdfs:label "paper"@en ;
    rdfs:comment "An official document that provides information about a particular subject or a detailed account of issues, policies or outcomes of, for example, inquiries or scientific investigations. Its structures vary widely across organizations and traditions."@en ;
    rdfs:isDefinedBy <https://w3id.org/un/ontology/undo> ;
    rdfs:subClassOf :Document .

:Relation a owl:Class ;
    rdfs:label "relation"@en ;
    rdfs:comment "Something that allows one to link a proponent entity to a receiver entity according to a specific semantics - e.g. saying that a document (proponent) cites (semantics) another document (receiver), or that an organization (proponent) approves (semantics) a certain document (receiver), etc."@en ;
    rdfs:isDefinedBy <https://w3id.org/un/ontology/undo> ;
    rdfs:subClassOf [ a owl:Restriction ;
            owl:cardinality "1"^^xsd:nonNegativeInteger ;
            owl:onProperty :hasProponent ],
        [ a owl:Restriction ;
            owl:cardinality "1"^^xsd:nonNegativeInteger ;
            owl:onProperty :hasReceiver ],
        [ a owl:Restriction ;
            owl:cardinality "1"^^xsd:nonNegativeInteger ;
            owl:onProperty :hasSemantics ],
        <https://w3id.org/akn/ontology/allot/Concept> .

:Value a owl:Class ;
    rdfs:label "value"@en ;
    rdfs:comment "Something that can be held by an entity (e.g. a particular role or status)."@en ;
    rdfs:isDefinedBy <https://w3id.org/un/ontology/undo> ;
    rdfs:subClassOf dul:Concept .

<https://w3id.org/akn/ontology/allot/Event> a owl:Class ;
    rdfs:isDefinedBy <https://w3id.org/akn/ontology/allot> .

:Step a owl:Class ;
    rdfs:label "step"@en ;
    rdfs:comment "An atomic unit of a workflow that involves some input entity needed to complete the step, and produces some outcomes, such as a document."@en ;
    rdfs:isDefinedBy <https://w3id.org/un/ontology/undo> ;
    rdfs:subClassOf [ a owl:Restriction ;
            owl:allValuesFrom :Step ;
            owl:onProperty pwo:hasNextStep ],
        [ a owl:Restriction ;
            owl:allValuesFrom <https://w3id.org/akn/ontology/allot/Reference> ;
            owl:onProperty pwo:needs ],
        [ a owl:Restriction ;
            owl:allValuesFrom <https://w3id.org/akn/ontology/allot/Reference> ;
            owl:onProperty pwo:produces ],
        [ a owl:Restriction ;
            owl:allValuesFrom :Action ;
            owl:onProperty <http://www.ontologydesignpatterns.org/cp/owl/taskexecution.owl#isExecutedIn> ],
        pwo:Step,
        <https://w3id.org/akn/ontology/allot/Concept> .

:Communication a owl:Class ;
    rdfs:label "communication"@en ;
    rdfs:comment "A document containing an official communication used to formally inform the UN community of events and of the outcome of non-UN meetings, to transmit reports or communications, and for a variety of other purposes. Its structures vary widely across organizations and traditions but generally assume the format of a formal communication with title and content in unnumbered paragraphs."@en ;
    rdfs:isDefinedBy <https://w3id.org/un/ontology/undo> ;
    rdfs:subClassOf :Document .

:Language a owl:Class ;
    rdfs:label "language"@en ;
    rdfs:comment "A particular language adopted by the United Nation for publishing their documents (e.g. Arabic, Chinese, English, French, Russian, Spanish)."@en ;
    rdfs:isDefinedBy <https://w3id.org/un/ontology/undo> ;
    rdfs:subClassOf <http://purl.org/dc/terms/LinguisticSystem>,
        <https://w3id.org/akn/ontology/allot/Concept> .

<https://w3id.org/akn/ontology/allot/Reference> a owl:Class ;
    rdfs:isDefinedBy <https://w3id.org/akn/ontology/allot>,
        <https://w3id.org/un/ontology/undo> .

<https://w3id.org/akn/ontology/allot/Concept> a owl:Class ;
    rdfs:isDefinedBy <https://w3id.org/akn/ontology/allot> ;
    rdfs:subClassOf skos:Concept .

:Document a owl:Class ;
    rdfs:label "document"@en ;
    rdfs:comment "A document of a specific kind (e.g. normative documents, legal documents, etc.) published by someone for certain reasons."@en ;
    rdfs:isDefinedBy <https://w3id.org/un/ontology/undo> ;
    rdfs:subClassOf [ a owl:Restriction ;
            owl:onProperty <https://w3id.org/akn/ontology/allot/hasRealization> ;
            owl:someValuesFrom :DocumentVersion ],
        <https://w3id.org/akn/ontology/allot/FRBRWork> .

:NormativeDocument a owl:Class ;
    rdfs:label "normative document"@en ;
    rdfs:comment "Formal provision concerning commands, recommendations, opinions or expressions of will issued or entered into by a principal or a subsidiary organ or other empowered bodies. Usually, it is articulated in hierarchical structures, in which the text is subdivided into higher and lower subdivisions."@en ;
    rdfs:isDefinedBy <https://w3id.org/un/ontology/undo> ;
    rdfs:subClassOf :Document .

<https://w3id.org/un/ontology/undo> a owl:Ontology ;
    rdfs:label "UNDO"@en ;
    dc:contributor "HLCM Working Group on Document Standards of the United Nations",
        "Silvio Peroni (http://orcid.org/0000-0003-0530-4305)" ;
    dc:description """The parliamentary, normative and judicial documents published by the United Nations system of organizations, from now on “UN Documents”, are full of references to real-world objects and concepts, such as other documents, people, organizations, legal terms, and roles. Such entities are linked with the actual content of the document, even by means of different terms being the UN documents often issued in several official languages.

The HLCM Working Group on Document Standards was tasked to define a common set of guidelines for the semantic mark-up of UN documents based on the [Akoma Ntoso standard](http://akomantoso.org) of the LegalDocumentML Technical Committee of the Organization for the Advancement of Structured Information Standards (OASIS), which has defined an open document standard for parliamentary, legislative, administrative, executive, and judicial documents.

The Akoma Ntoso ontology is centred on the concept of document, which is considered in a very precise way through the specification of the Functional Requirements for Bibliographic Records (FRBR) standard of the International Federation of Library Associations (IFLA). The Akoma Ntoso ontology structure is divided in two main categories:

* document classes: focused on all entities that represent the different aspects of a document as intellectual creation, the forms (versions, translations, etc.) that it may take and its physical embodiment (PDF, XML, HTML, paper, etc.);

* non-document classes: focused on two different aspects, namely who is responsible for the production of the content (organization, person, etc.) and what the content is about (concept, object, event, locations, roles, deliberation steps, etc.).

For the document classes Akoma Ntoso has defined a set of prescriptive / canonical classes and sub-classes modelled on the FRBR conceptualization of documents. These classes are referred by with specific XML tags (prefixed by “FRBR”) in Akoma Ntoso documents. For non-document classes of parliamentary and legal matters, the Akoma Ntoso specifications rather than defining the ontology, which could be overly wide and all-encompassing due to rather huge and all-encompassing issues that legal and parliamentary documents deal with, specify a very broad set of general guidelines that an ontology should conform to in order to be used in conjunction with Akoma Ntoso documents. These informal guidelines are referred by with specific XML tags (prefixed by “TLC”) in Akoma Ntoso documents, each referring to a particular informal top level class (TLC), i.e. that is not defined by means of a formal language such as logics.

The United Nations System Document Ontology (UNDO, https://w3id.org/un/ontology/undo) is an OWL 2 DL ontology that aims at providing a framework for the formal description of all entities and the relations that can exist among them in UN Documents, description that is not provided by Akoma Ntoso. The idea behind the development of this model is to have a mechanism for sharing data about documents and their content in RDF format in an interchangeable way and, eventually, extended by the various agencies of the United Nations to meet their own domain specific requirements.

It is worth mentioning that UNDO and the [official UN document describing it](https://w3id.org/un/document/undo) are living artefacts, and they have been drafted in the context of the HLCM Working Group on Document Standards under the technical supervision of [Silvio Peroni](https://orcid.org/0000-0003-0530-4305). They will be subject to regular updates to incorporate new developments and requirements.

Currently, UNDO is able to describe the following entities:

* documents and their versions (e.g. in different languages);

* several relevant document types, organized in a taxonomy;

* mentions to specific entities introduced in documents;

* relations among entities (i.e. both documents and the entities they mention);

* annotations, in order to link any RDF description to a particular document;

* terms, i.e. tokens as they can appear in a text, and their semantics;

* values that can change in time and context (such as agents’ roles and document statuses);

* workflows and their executions. 

The following figure contains a [Graffoo diagram](http://www.essepuntato.it/graffoo) that provides an overview of the class and properties introduced in UNDO.

![A Graffoo diagram of UNDO](undo.png)

The current version of the ontology imports several ontologies:

* [ALLOT](https://w3id.org/akn/ontology/allot) provides a formal implementation of Akoma Ntoso Top Level Classes (TLCs) in OWL 2 DL, so as to make available a vocabulary for enabling the integration of heterogeneous legal knowledge-bases based on Akoma Ntoso documents;

* [Publishing Workflow Ontology](http://purl.org/spar/pwo) provides a framework for characterising the main stages in the workflow associated with the publication of a document;

* [Time-indexed Value in Context](http://www.essepuntato.it/2012/04/tvc) is an ontology pattern that allows one to describe scenarios in which someone (e.g., a person) has a value (e.g., a particular role) during a particular time and for a particular context;

* [Time Interval](http://www.ontologydesignpatterns.org/cp/owl/timeinterval.owl) is an ontology pattern that enables the description of period of times characterised by a starting date and an ending date;

* [Web Annotation Ontology](https://www.w3.org/ns/oa) is a set of RDF classes, predicates and named entities that are used by the [Web Annotation Data Model](https://www.w3.org/TR/annotation-model/) for creating annotations in RDF;

In addition to these ontologies, UNDO is also aligned with entities defined in external ontologies and vocabularies, in particular:

* [Dublin Core Metadata Terms](http://purl.org/dc/terms/) is an ontology implementing all the metadata terms maintained by the Dublin Core Metadata Initiative, including properties, vocabulary encoding schemes, syntax encoding schemes, and classes;

* [FaBiO](http://purl.org/spar/fabio) is an ontology for recording and publishing on the Semantic Web bibliographic records of scholarly endeavours;

* [FOAF](http://xmlns.com/foaf/0.1/) is an ontology for describing people and their relations with other people, documents, and other information objects;

* [FRBR DL](http://purl.org/spar/frbr) is an expression in OWL 2 DL of the basic concepts and relations described in the IFLA report on the [Functional Requirements for Bibliographic Records (FRBR)](http://www.ifla.org/publications/functional-requirements-for-bibliographic-records), also described in [Ian Davis's RDF vocabulary](http://vocab.org/frbr/core);

* [ISO 639-1](http://id.loc.gov.vocabulary/iso693-1) is a vocabulary describing the first part of the ISO 639 international-standard language-code family;

* [LKIF Core: Action](http://www.estrellaproject.org/lkif-core/action.owl) is an ontology for representing actions in general, i.e. processes which are performed by some agent;

* [LKIF Core: Role](http://www.estrellaproject.org/lkif-core/role.owl) is an ontology for describing typology of roles (epistemic roles, functions, person roles, organisation roles);

* [PRO](http://purl.org/spar/pro) is an ontology describing possible roles in the publication process, or in other scholarly activities or situations, held by particular agent;

* [PSO](http://purl.org/spar/pso) is an ontology for characterizing the publication status of a document or other publication entity at each of the various stages in the publishing process;

* [SKOS](https://www.w3.org/TR/skos-reference/) is a common data model for sharing and linking knowledge organization systems via the Web.

A full version of UNDO, where all the aforementioned ontologies have been imported formally within the ontology, is available at https://w3id.org/akn/ontology/undo-imports, so as to enable advanced automatic reasoning and classification.

In addition, it is also aligned to two important foundational ontologies, i.e. the [Basic Formal Ontology (BFO)](http://purl.obolibrary.org/obo/bfo/2.0/bfo.owl) and the [Descriptive Ontology for Linguistic and Cognitive Engineering (DOLCE)](http://www.ontologydesignpatterns.org/ont/dul/DUL.owl). This alignment is crucial since it enables a reusability of the model in different contexts and domains (e.g. BFO is already used in several models adopted by the United Nations), and it also provides a methodological organization of all the entities introduced in UNDO.

The next subsections provide a quick overview of all the entities defined, some exemple of usage, and the query that UNDO can answer.

### Documents and their versions

Several existing models have tried to explain the difference between documents and their versions. By means of ALLOT – which in turn uses a well-known and robust model for characterizing bibliographic metadata, the Functional Requirements for Bibliographic Records (FRBR) – UNDO separates documents (e.g. UN resolution A/RES/50/100) and versions (e.g. language versions) in two specific and distinct layers, characterized by two classes: `undo:Document` and `undo:DocumentVersion`. 

On the one hand, following the FRBR classification, the former class maps on the FRBR Work level, and it describes the document essence, independently from the revisions and/or translations that can characterizes it in time. On the other hand, the class for document versions maps on the FRBR Expression level, and it is used for pointing to specific realizations of a document characterized by a particular and fixed content. For instance, a draft in English, an amended version of that draft, a translation in French are all different versions (i.e. FRBR Expressions) of the same document (i.e. FRBR Work).

There are four properties available in UNDO that can be used for defining relations among these classes:

* property `allot:hasRealization`, which links a document with its versions;

* property `frbr:revision`, which links a specific version to another version of it (e.g. a draft that has been amended and revised) –  it is possible to add appropriate information concerning which document produced the revision, when the new revision is effective, and the list of the revisions produced by means of some of the models that have been aligned/imported by UNDO, i.e. PWO and FaBiO;

* property `dcterms:language`, which allows one to specify the language associated to the specific version in consideration – the link between translations in different languages can be linked by means of the property `frbr:translation` defined in FRBR DL to which UNDO aligns;

* property `frbr:transformation`, used for describing documents that are transformed somehow in another original document (even of another type – see the following section) in a sufficient degree to warrant their being considered as new works (e.g. when the General Assembly publish a new resolution from a draft provided by someone).

It is worth mentioning that, in case it is needed, the characterization of the document components should be handled by means of the Document Components Ontology (DoCO, http://purl.org/spar/doco).


### Document types

While, on the one hand, the dichotomy between documents and their versions is an important aspect to address, on the other hand it is also crucial to provide an appropriate taxonomy of defining document types, so as to allow one to describe them appropriately. In UNDO, the class `undo:Document` includes several subclasses taking care of providing appropriate descriptions for the main United Nations documents (`undo:Resolution`, `undo:Constitution`, `undo:Standard`, etc.). Each document type is accompanied by a natural language description clarifying its role.


### Documents mentioning other entities

The parliamentary, normative and legal documents published by the United Nations System of Organizations are full of references to real-world objects and concepts, such as other documents, people, organizations, legal terms, and roles. UNDO makes available the property `allot:mentions` for linking a document (or one specific version of it) to a particular entity (defined by the class `allot:Reference`) that is mentioned within (e.g. that the resolution A/RES/50/100 mentions the Government of Turkey). This property allows one to build a sophisticated network of references to entities that enables the cross-navigation between documents and other related resources.


### Relations

While the aforementioned property is important, on the one hand, it does not allow one to specify the particular semantics justifying a particular mention of an entity in a document – e.g., recalling the example in the previous section, the reasons why the resolution A/RES/50/100 mentions the Government of Turkey. On the other hand, other relevant relations between non-document entities, that are by reading the natural language argumentations carried by the document content, cannot be described – e.g. the sentence of the aforementioned resolution where “the General Assembly reiterates its gratitude to the Government of Turkey”. Since it is not possible to define all the kinds of relations that could be hidden behind the content of any United Nations document, UNDO makes available a mechanism for defining such relations in a flexible way without changing the actual terminological specification of the ontology, i.e. its TBox.

Thus we have chosen to define relations between entities by means of a particular class, i.e. `undo:Relation`, so as to enable the specification of the semantics of such relations by using individuals of the class `allot:Concept`. This approach is quite robust, since if one need a new semantics for a relation s/he has only to add a new individual to the class allot:Concept, thus modifying only the ABox of the ontology and, implicitly, reducing the chances of introducing inconsistencies. In addition, this approach is very flexible, since it allows one to extend the set of relations applicable between entities every time there is a specific need.

In particular, the properties that can be used with the instances of the class undo:Relation are introduced as follows:

* the property `undo:hasProponent`, which is used for identifying the subject entity of a relation (e.g. the “General Assembly” described in the sentence “the General Assembly reiterates its gratitude to the Government of Turkey”);

* the property `undo:hasReceiver`, which is used for identifying the object entity of a relation (e.g. the “Government of Turkey”, in the previous example);

* the property `undo:hasSemantics`, which is used for specifying the particular concept defining the semantics of the relation.


### Annotations to documents

By reading a document content, several people can derive different (even contrasting) interpretations upon the same text. For instance, the same sentence, e.g. “Encourages all relevant non-governmental organizations […] to participate in and contribute to the Conference” can be read as an invitation or as a reproach for having not doing any action yet. Therefore, it is important to have some mechanism for allowing the existence of all these different interpretations in a way that is understandable and still consistent from an ontological perspective.

For this reason, UNDO reuses the framework defined in the Web Annotation Ontology that allows one to annotate documents (or even portions of them) by means of another entity, such as a relation as introduced in the previous subsection. In particular, every annotation in UNDO is defined as an individual of the class undo:Annotation, and the following properties are used to linking an entity to the document its annotate:

* the property `oa:hasBody` is used to specify the body of the annotation to be attached to the document;

* the property `oa:hasTarget` is used to indicate the particular document (described according to any of the available FRBR levels) to which the annotation is specified.

In addition, each document (or any of its parts) can be explicitly annotated (using instances of `undo:Annotation`) by someone with all these relations in order to create a formal connection between the text and the entities its introduces.


### Terms and their semantics

Broadly speaking, terms are words or groups of words whose meanings are defined in a formal and precise manner by means of specific concepts. Thus, terms can refer to nouns (e.g. “computer keyboard”), verbs (e.g. “decide”), persons (e.g. “John”), cities (e.g. “New York”), etc., they can share the same textual content while being polysemous (e.g. the city “Paris” and the person “Paris”), they can refer to the same meaning (e.g. the third person verb “decides” in English and its related in Spanish, “decide”), and so on.

In UNDO the class `allot:Term` is used to define terms, while the property `undo:hasRelatedConcept` enables one to link a term to the concept (introduced by the class `allot:Concept`) defining the meaning of the term in consideration.


### Values, time and context
Several kinds of objects can be involved in situations (undo:ValueInTimeAndContext) describing them as holding a certain value (tvc:withValue) associated for a specific interval (tvc:atTime) or according to a specific context (tvc:withinContext). For instance, agents having a particular role (e.g. being the President of the United Nations General Assembly for the whole 2016) or documents holding particular status (e.g. a document that has been under-review from September 2016 to October 2016) in a specific time and/or related to a particular context are examples for these situations.

In UNDO these situations can be described by means of the class `undo:ValueInTimeAndContext`, which introduces the framework defined by the Time-indexed Value in Time (TVC) ontology pattern for defining in details all the aforementioned temporal and contextual aspects. In particular, it allows one to specify:

* the entity holding such value (e.g. an agent or a document) by means of the property `tvc:hasValue`;

* the value held (e.g. a role or a status) by means of the property `tvc:withValue`;

* the time defining when such value is held (e.g. from 2006 to 2015) using the property `tvc:atTime`;

* the context to which the scenario applies (e.g. the United Nations General Assembly) using the property `tvc:withinContext`.


### Workflows and their executions

Keeping track of the processes concerning the creation and modification of documents is a crucial task to address in the legal and legislative domain. Each of these processes, commonly called workflow, is actually composed by a sequence of steps. Each step is responsible to produce some outputs (e.g. a review) starting from some inputs (e.g. a document). 

In UNDO, workflows can be described from two different points of view, by reusing the framework implemented in the Publishing Workflow Ontology (PWO). On the one hand, there is the declaration of the workflow schema, or simply the workflow (`undo:Workflow`), which is how a specific process (e.g. the publication of a document) is organized in sequential steps (`undo:Step`), where each step:

* has a specific type (property `undo:hasStepType`);

* needs some input (property `pwo:needs`);

* produces a particular output (property `pwo:produces`). 

On the other hand, each particular execution of a workflow (undo:WorkflowExecution) is a specific entity per se, it is usually composed by sets of actions (undo:Action), and each action:

* addresses (part of) a particular step defined in the workflow in consideration (property taskex:executesTask);

* involves entities as participants (`part:hasParticipant`);

* is executed within a particular interval (`pwo:happened`).

It is worth mentioning that this module of UNDO is able to describe the full characterization that Akoma Ntoso provides in its specification about document workflows and lifecycles –  the latter by means of the class `undo:Lifecycle`.



### Example of use

UNDO can be used for modelling several scenarios that are typical to the documents published by the United Nations (e.g. UN Resolutions). In the following subsections we introduce some of them, and we accompany them with exemplar instantiations. 

The prefixes that are used in all the examples provided below are defined as follows:

    @prefix : <https://w3id.org/akn/data/undo/> .
    @prefix undo: <https://w3id.org/akn/ontology/undo/> .
    @prefix allot: <https://w3id.org/akn/ontology/allot/> .
    @prefix owl: <http://www.w3.org/2002/07/owl#> .
    @prefix dcterms: <http://purl.org/dc/terms/> .
    @prefix lan: <http://id.loc.gov/vocabulary/iso639-1/> .
    @prefix oa: <http://www.w3.org/ns/oa#> .
    @prefix part: <http://www.ontologydesignpatterns.org/cp/owl/participation.owl#> .
    @prefix pwo: <http://purl.org/spar/pwo/> .
    @prefix taskex: <http://www.ontologydesignpatterns.org/cp/owl/taskexecution.owl#> .
    @prefix ti: <http://www.ontologydesignpatterns.org/cp/owl/timeinterval.owl#> .
    @prefix frbr: <http://purl.org/vocab/frbr/core#> .
    @prefix tvc: <http://www.essepuntato.it/2012/04/tvc/> .



#### Scenario 1

In the preface of the UN resolution A/RES/50/100 of 2 February 1996 there are references to:

1. the UN resolution A/RES/47/180 of 22 December 1992;
2. the Government of Turkey;
3. the United Nations Conference on Human Settlements (Habitat II).

```
:a-res-50-100-1996-02-02 a undo:Resolution ;
    allot:mentions
        :a-res-47-180-1992-12-22 ,
        :government-of-turkey ,
        :habitat-ii .

:a-res-47-180-1992-12-22 a undo:Resolution .
:government-of-turkey a allot:Organization .
:habitat-ii a allot:Event .
```


#### Scenario 2

According to the content of the UN resolution A/RES/50/100 of 2 February 1996, the General Assembly:

1. recalls the resolution A/RES/47/180 of 22 December 1992;
2. reiterates its gratitude to the Government of Turkey;
3. notes the progress that has been made so far in the preparations for the United Nations Conference on Human Settlements (Habitat II).

```
:a-res-50-100-1996-02-02 a undo:Resolution .
:a-res-47-180-1992-12-22 a undo:Resolution .
:general-assembly a allot:Organization .
:organization a allot:Organization .
:government-of-turkey a allot:Organization .
:habitat-ii a allot:Event .
:recall a allot:Concept .
:reiterate-its-gratitude a allot:Concept .
:note-the-progress a allot:Concept .

# This relation describes the General Assembly recalling the
 # resolution A/RES/47/180.
:relation-1 a undo:Relation ;
    undo:hasProponent :general-assembly ;
    undo:hasSemantics :recall ;
    undo:hasReceiver :a-res-47-180-1992-12-22 .

# This relation describes the General Assembly reiterating its gratitude 
 # to the Government of Turkey.
:relation-2 a undo:Relation ;
    undo:hasProponent :general-assembly ;
    undo:hasSemantics :reiterate-its-gratitude ;
    undo:hasReceiver :government-of-turkey .

# This relation describes the General Assembly noting the progress for the 
 # preparation of Habitat II.
:relation-3 a undo:Relation ;
    undo:hasProponent :general-assembly ;
    undo:hasSemantics :note-the-progress ;
    undo:hasReceiver :habitat-ii .

# The following are a three annotations that attached the aforementioned 
# relations to the resolution A/RES/50/100 from which they have been
 # extracted.
:annotation-1-a-res-50-100-1996-02-02 a undo:Annotation ;
    oa:hasBody :relation-1 ;
    oa:hasTarget :a-res-50-100-1996-02-02 .

:annotation-2-a-res-50-100-1996-02-02 a undo:Annotation ;
    oa:hasBody :relation-2 ;
    oa:hasTarget :a-res-50-100-1996-02-02 .

:annotation-3-a-res-50-100-1996-02-02 a undo:Annotation ;
    oa:hasBody :relation-3 ;
    oa:hasTarget :a-res-50-100-1996-02-02 .
```

#### Scenario 3

The UN resolution A/RES/50/100 has been published in six different languages. The term "decides" has been used twice in the English version, and, in parallel, the term "decide" has been used twice in the Spanish version. Both the terms actually refers to the same higher-level concept of taking a decision, even if this aspect has not been made formally explicit in the document itself.

```
# The resolution A/RES/50/100 that has been made available in two different
# versions according to two languages.
:a-res-50-100-1996-02-02 a undo:Resolution ;
    allot:hasRealization
        :a-res-50-100-1996-02-02-en ,
        :a-res-50-100-1996-02-02-es .

# The English version of the resolution.
:a-res-50-100-1996-02-02-en a undo:DocumentVersion ;
    dcterms:language lan:en .

# The Spanish version of the resolution.
:a-res-50-100-1996-02-02-es a undo:DocumentVersion ;
    dcterms:language lan:es .

# The definition of an English term describing the concept of 
# ‘taking a decision’ and two distinct annotation that attach it
# to the same English version of the resolution – since the term
# appears twice in the document.
:decides a allot:Term ;
    undo:hasRelatedConcept :taking-a-decision .

:annotation-1-a-res-50-100-1996-02-02-en a undo:Annotation ;
    oa:hasBody :decides ;
    oa:hasTarget :a-res-50-100-1996-02-02-en .

:annotation-2-a-res-50-100-1996-02-02-en a undo:Annotation ;
    oa:hasBody :decides ;
    oa:hasTarget :a-res-50-100-1996-02-02-en .

# A similar description of the previous term, but by means of its Spanish
# translation.
:decide a allot:Term ;
    undo:hasRelatedConcept :taking-a-decision .

:annotation-1-a-res-50-100-1996-02-02-es a undo:Annotation ;
    oa:hasBody :decide ;
    oa:hasTarget :a-res-50-100-1996-02-02-es .

:annotation-2-a-res-50-100-1996-02-02-es a undo:Annotation ;
    oa:hasBody :decide ;
    oa:hasTarget :a-res-50-100-1996-02-02-es .

:taking-a-decision a allot:Concept .
```

#### Scenario 4

Giorgio Napolitano has been President of Italy for the first time from the 15th of May 2006 to the 22th of April 2013, when he resigned. He has been elected again on the 22th of April 2013, and he has been President of Italy for the second time by the 14th of January 2015, when he resigned for the second time. He has been substituted by Sergio Mattarella, who starts his mandate as President of Italy on the 3rd of February 2015, formerly judge of the Constitutional Court of Italy from the 11th of October 2011 to the 2nd of February 2015.

```
# Giorgio Napolitano who has been President of Italy in two distinct periods:
# the first one from 2006 to 2013, and the second one from 2013 to 2015.
:giorgio-napolitano a undo:Agent ;
    tvc:hasValue
        :giorgio-napolitano-president-of-italy-2006-2013 ,
        :giorgio-napolitano-president-of-italy-2013-2015 .

# First mandate of Giorgio Napolitano as President of Italy.
:giorgio-napolitano-president-of-italy-2006-2013 a undo:ValueInTimeAndContext ;
    tvc:withValue :president ;
    tvc:atTime :2006-2013 ;
    tvc:withinContext :italy .

# Second mandate of Giorgio Napolitano as President of Italy.
:giorgio-napolitano-president-of-italy-2013-2015 a undo:ValueInTimeAndContext ;
    tvc:withValue :president ;
    tvc:atTime :2013-2015 ;
    tvc:withinContext :italy .

:president a allot:Role .

# The intervals defining the two mandates of Giorgio Napolitano as
# President of Italy.
:2006-2013 a undo:Interval ;
    ti:hasIntervalStartDate "2006-05-15T00:00:00"^^xsd:dateTime ;
    ti:hasIntervalEndDate "2013-04-22T00:00:00"^^xsd:dateTime .

:2013-2015 a undo:Interval ;
    ti:hasIntervalStartDate "2013-04-22T00:00:00"^^xsd:dateTime ;
    ti:hasIntervalEndDate "2015-01-14T00:00:00"^^xsd:dateTime .

:italy a allot:Reference .

# Sergio Mattarella in relation to its roles of judge of the Constitutional
# Court of Italy before becoming President of Italy in 2015.
:sergio-mattarella a undo:Agent ;
    tvc:hasValue
        :sergio-mattarella-judge-constitutional-court-of-italy-2011-2015 ,
        :sergio-mattarella-president-of-italy-since-2015.

# Sergio Mattarella acting as a judge.
:sergio-mattarella-judge-constitutional-court-of-italy-2011-2015 a undo:ValueInTimeAndContext ;
    tvc:withValue :judge ;
    tvc:atTime :2011-2015 ;
    tvc:withinContext :constitutional-court-of-italy .

# Sergio Mattarella acting as President of Italy.
:sergio-mattarella-president-of-italy-since-2015 a undo:ValueInTimeAndContext ;
    tvc:withValue :president ;
    tvc:atTime :since-2015 ;
    tvc:withinContext :italy .

# The intervals related to Sergio Mattarella’s roles.
:2011-2015 a undo:Interval ;
    ti:hasIntervalStartDate "2011-10-11T00:00:00"^^xsd:dateTime ;
    ti:hasIntervalEndDate "2015-02-03T00:00:00"^^xsd:dateTime .

:since-2015 a undo:Interval ;
    ti:hasIntervalStartDate "2015-02-03T00:00:00"^^xsd:dateTime .

:constitutional-court-of-italy a allot:Reference .

:judge a allot:Role .
```


#### Scenario 5

A document has been in drafting from the 14th of May to the 14th of June 2016. Then, it has been under revision for the following two months, and finally published on the 1st of September 2016.

```
# The three statuses associated to the document.
:a-document a undo:Document ;
    tvc:hasValue
        :document-in-drafting ,
        :document-under-revision ,
        :document-published .

# The status of being in drafting.
:document-in-drafting a undo:ValueInTimeAndContext ;
    tvc:withValue :in-drafting ;
    tvc:atTime :in-drafting-interval .

# The status of being under revision.
:document-under-revision a undo:ValueInTimeAndContext ;
    tvc:withValue :under-revision ;
    tvc:atTime :under-revision-interval .

# The status of being published.
:document-published a undo:ValueInTimeAndContext ;
    tvc:withValue :published ;
    tvc:atTime :published-interval .

# The intervals defining how long the aforementioned status have been  
# assigned to the document in consideration.
:in-drafting-interval a undo:Interval ;
    ti:hasIntervalStartDate "2016-05-14T00:00:00"^^xsd:dateTime ;
    ti:hasIntervalEndDate "2016-06-14T00:00:00"^^xsd:dateTime .

:under-revision-interval a undo:Interval ;
    ti:hasIntervalStartDate "2016-06-14T00:00:00"^^xsd:dateTime ;
    ti:hasIntervalEndDate "2016-08-14T00:00:00"^^xsd:dateTime .

:published-interval a undo:Interval ;
    ti:hasIntervalStartDate "2016-09-01T00:00:00"^^xsd:dateTime .

:in-drafting a undo:Status .

:under-revision a undo:Status .

:published a undo:Status .
```

#### Scenario 6

The publication of a document should go through four phases, or steps: 

1. writing, which will produce a document;
2. review, that will produce comments starting from the input document;
3. revision, that will produce a new version of the previous document corrected considering the comments produced by the previous step; 
4. publication, which will assign the "published" status to that document. 

```
# The four steps composing the workflow.
:publication a undo:Workflow ;
    pwo:hasStep
        :step-1 ,
        :step-2 ,
        :step-3 ,
        :step-4 .

# The definition of each step according to its type, including the link to 
# the other step that follows the one in consideration (in any).
:step-1 a undo:Step ;
    undo:hasStepType :write ;
    pwo:hasNextStep :step-2 .

:write a undo:StepType .

:step-2 a undo:Step ;
    undo:hasStepType :review ;
    pwo:hasNextStep :step-3 .

:review a undo:StepType .

:step-3 a undo:Step ;
    undo:hasStepType :revise ;
    pwo:hasNextStep :step-4 .

:revise a undo:StepType .

:step-4 a undo:Step ;
    undo:hasStepType :publish .

:publish a undo:StepType .
```


#### Scenario 7

The Assistant of a Representative writes the first draft of a resolution from the 1st of March 2017 to the 5th of March 2017. On the 7th of March, the Representative revises it, and extends the introduction. From the 9th of March to the 10th of March, Assistant of the Representative finalises the document. On the 11th of March, the State Member makes it available for review.

On the 12th of March, the Office of the Presidency of the General Assembly read the draft. From the 13th of March to the 20th of March, the Office of the Presidency of the General Assembly writes a comment highlighting issues. The comment is then made available to the President of the General Assembly on the 21st of March.

From the 22nd to the 27th of March, the Committee Number 1 revises the draft and addresses the main issues raised by the Office of the Presidency of the General Assembly. On the 28th, the draft is sent to the General Assembly.

The General Assembly approves and publishes the resolution on the 31st of March.

```
# A document that will become a resolution after the workflow execution, 
# accompanied by all the versions that have been created during the process.
:future-resolution a undo:Document ;
    allot:hasRealization
        :assistant-first-draft-resolution ,
        :member-rep-extended-introduction-first-draft ,
        :final-first-draft ,
        :revised-draft .

# The first draft created by the assistant of the representative, and
# the related action of writing it.
:assistant-member-rep a undo:Agent .
:assistant-first-draft-resolution a undo:DocumentVersion .
:2017-03-01_05 a undo:Interval ;
     ti:hasIntervalStartDate "2017-03-01T00:00:00"^^xsd:dateTime ;
     ti:hasIntervalEndDate "2017-03-05T23:59:59"^^xsd:dateTime .
:writing-first-draft a undo:Action ;
    taskex:executesTask :step-1 ;
    part:hasParticipant
        :assistant-member-rep ,
        :assistant-first-draft-resolution ;
    pwo:happened :2017-03-01_05 .

# The revision proposed by the representative, who extended
# the previous draft.
:member-rep a undo:Agent .
:assistant-first-draft-resolution 
    frbr:revision :member-rep-extended-introduction-first-draft .
:member-rep-extended-introduction-first-draft a undo:DocumentVersion .
:2017-03-07 a undo:Interval ;
     ti:hasIntervalStartDate "2017-03-07T00:00:00"^^xsd:dateTime ;
     ti:hasIntervalEndDate "2017-03-07T23:59:59"^^xsd:dateTime .
:extending-first-draft a undo:Action ;
    taskex:executesTask :step-1 ;
    part:hasParticipant 
        :member-rep ,
        :assistant-first-draft-resolution ,
        :member-rep-extended-introduction-first-draft ;
    pwo:happened :2017-03-07 .

# The submission of the draft by the state member to the General Assembly.
:member-rep-extended-introduction-first-draft
    frbr:revision :final-first-draft .
:final-first-draft a undo:DocumentVersion .
:2017-03-09_10 a undo:Interval ;
     ti:hasIntervalStartDate "2017-03-09T00:00:00"^^xsd:dateTime ;
     ti:hasIntervalEndDate "2017-03-10T23:59:59"^^xsd:dateTime .
:revision-first-draft a undo:Action ;
    taskex:executesTask :step-1 ;
    part:hasParticipant 
        :assistant-member-rep ,
        :member-rep-extended-introduction-first-draft ,
        :final-first-draft ;
    pwo:happened :2017-03-09_10 .

:member a undo:Agent .
:2017-03-11 a undo:Interval ;
     ti:hasIntervalStartDate "2017-03-11T00:00:00"^^xsd:dateTime ;
     ti:hasIntervalEndDate "2017-03-11T23:59:59"^^xsd:dateTime .
:making-available-first-draft a undo:Action ;
    taskex:executesTask :step-1 ;
    part:hasParticipant 
        :member ,
        :final-first-draft ;
    pwo:happened :2017-03-11 .

:step-1 pwo:produces :final-first-draft .

# The reading done by the Office of the Presidency of the General Assembly
# to the draft submitted.
:office-presidency-ga a undo:Agent .
:2017-03-12 a undo:Interval ;
     ti:hasIntervalStartDate "2017-03-12T00:00:00"^^xsd:dateTime ;
     ti:hasIntervalEndDate "2017-03-12T23:59:59"^^xsd:dateTime .
:reading-final-first-draft a undo:Action ;
    taskex:executesTask :step-2 ;
    part:hasParticipant 
        :office-presidency-ga ,
        :final-first-draft ;
    pwo:happened :2017-03-12 .

# The creation of a comment that explains issues and proposes modification
# to the submitted draft. 
:2017-03-13_20 a undo:Interval ;
     ti:hasIntervalStartDate "2017-03-13T00:00:00"^^xsd:dateTime ;
     ti:hasIntervalEndDate "2017-03-20T23:59:59"^^xsd:dateTime .
:comment a undo:Document ;
    allot:hasRealization :comment-content .
:comment-content a undo:DocumentVersion .
:writing-comment a undo:Action ;
    taskex:executesTask :step-2 ;
    part:hasParticipant 
        :office-presidency-ga ,
        :final-first-draft ,
        :comment-content ;
    pwo:happened :2017-03-13_20 .

# The comment is made available by the President of the General Assembly.
:president-ga a undo:Agent .
:2017-03-21 a undo:Interval ;
     ti:hasIntervalStartDate "2017-03-12T00:00:00"^^xsd:dateTime ;
     ti:hasIntervalEndDate "2017-03-12T23:59:59"^^xsd:dateTime .
:making-available-comment a undo:Action ;
    taskex:executesTask :step-2 ;
    part:hasParticipant 
        :office-presidency-ga ,
        :president-ga ,
        :comment-content ;
    pwo:happened :2017-03-21 .

:step-2 
    pwo:needs :final-first-draft ;
    pwo:produces :comment-content .

# The Committee 1 revising the draft according to the comment.
:committee-1 a undo:Agent .
:final-first-draft
    frbr:revision :revised-draft .
:revised-draft a undo:DocumentVersion .
:2017-03-22_27 a undo:Interval ;
     ti:hasIntervalStartDate "2017-03-22T00:00:00"^^xsd:dateTime ;
     ti:hasIntervalEndDate "2017-03-27T23:59:59"^^xsd:dateTime .
:revision-final-first-draft a undo:Action ;
    taskex:executesTask :step-3 ;
    part:hasParticipant 
        :committee-1 ,
        :final-first-draft ,
        :comment ,
        :revised-draft ;
    pwo:happened :2017-03-22_27 .

# The Committee 1 that sends the revision o the General Assembly.
:ga a undo:Agent .
:2017-03-28 a undo:Interval ;
     ti:hasIntervalStartDate "2017-03-28T00:00:00"^^xsd:dateTime ;
     ti:hasIntervalEndDate "2017-03-28T23:59:59"^^xsd:dateTime .
:sending-revision a undo:Action ;
    taskex:executesTask :step-3 ;
    part:hasParticipant 
        :committee-1 ,
        :revised-draft ,
        :ga ;
    pwo:happened :2017-03-28 .

:step-3 
    pwo:needs :final-first-draft , :comment ;
    pwo:produces :revised-draft .

# The draft resolution is reconfigured as a proper resolution, that is thus
# published by the General Assembly.
:future-resolution
    frbr:transformation :resolution .
:resolution a undo:Resolution ;
    allot:hasRealization :resolution-text .
:resolution-text a undo:DocumentVersion .
:2017-03-31 a undo:Interval ;
     ti:hasIntervalStartDate "2017-03-31T00:00:00"^^xsd:dateTime ;
     ti:hasIntervalEndDate "2017-03-31T23:59:59"^^xsd:dateTime .
:approving-and-publishing-resolution a undo:Action ;
    taskex:executesTask :step-4 ;
    part:hasParticipant 
        :revised-draft ,
        :resolution-text ,
        :ga ;
    pwo:happened :2017-03-31 .

:step-4
    pwo:needs :revised-draft ;
    pwo:produces :resolution-text .

# The definition of the workflow execution, including all the actions
# that have been performed.
:publication-execution a undo:WorkflowExecution ;
    pwo:executes :publication ;
    pwo:involvesAction
        :writing-first-draft ,
        :extending-first-draft ,
        :revision-first-draft ,
        :making-available-first-draft ,
        :reading-final-first-draft ,
        :writing-comment ,
        :making-available-comment ,
        :revision-final-first-draft ,
        :sending-revision ,
        :approving-and-publishing-resolution .
```


### Competency questions

UNDO can be used for answering several questions related to the content of the documents published by the United Nations (e.g. UN Resolutions). In the following subsections we introduce some of them, and we accompany them with exemplar SPARQL queries. 

The prefixes that are used in all the SPARQL queries provided below are defined as follows:

    PREFIX : <https://w3id.org/akn/data/undo/>
    PREFIX allot: <https://w3id.org/akn/ontology/allot/>
    PREFIX oa: <http://www.w3.org/ns/oa#>
    PREFIX owl: <http://www.w3.org/2002/07/owl#>
    PREFIX undo: <https://w3id.org/akn/ontology/undo/>
    PREFIX ti: <http://www.ontologydesignpatterns.org/cp/owl/timeinterval.owl#>
    PREFIX tvc: <http://www.essepuntato.it/2012/04/tvc/>
    PREFIX frbr: <http://purl.org/vocab/frbr/core#>
    PREFIX pwo: <http://purl.org/spar/pwo/>
    PREFIX taskex: <http://www.ontologydesignpatterns.org/cp/owl/taskexecution.owl#>


#### Question 1

What are all the documents that refer to the UN resolution A/RES/47/180 of 22 December 1992?

    SELECT DISTINCT ?document
    WHERE {
        ?document allot:mentions :a-res-47-180-1992-12-22 .
    }

#### Question 2

What are all the entities referred by the UN resolution A/RES/50/100 of 2 February 1996?

    SELECT DISTINCT ?entity ?type
    WHERE {
        :a-res-50-100-1996-02-02 allot:mentions ?entity .
        ?entity a ?type .
        FILTER (?type != owl:NamedIndividual)
    }


#### Question 3

What are the documents that describes the General Assembly recalling the resolution A/RES/47/180 of 22 December 1992?

    SELECT DISTINCT ?document
    WHERE {
        ?rel a undo:Relation ;
            undo:hasProponent :general-assembly ;
            undo:hasSemantics :recall ;
            undo:hasReceiver :a-res-47-180-1992-12-22 .
        
        ?ann a undo:Annotation ;
            oa:hasBody ?rel ;
            oa:hasTarget ?document
    }


#### Question 4

What are all the terms that actually refer to the concept of taking a decision, and in which documents have been used?

    SELECT DISTINCT ?term ?document
    WHERE {
        ?term a allot:Term ;
            undo:hasRelatedConcept :taking-a-decision .
           
        ?ann a undo:Annotation ;
            oa:hasBody ?term ;
            oa:hasTarget ?document
    }


#### Question 5

What are the current roles of all the agents?

    SELECT DISTINCT ?agent ?role ?context
    WHERE {
        ?agent a undo:Agent ;
            tvc:hasValue ?value .
            
        ?value a undo:ValueInTimeAndContext ; 
            tvc:withValue ?role ;
            tvc:withinContext ?context .
        
        FILTER NOT EXISTS {
            ?value tvc:atTime/ti:hasIntervalEndDate ?time
        }
            
        ?role a allot:Role .
    }


#### Question 6

What roles have been held by Sergio Mattarella during his life?

    SELECT DISTINCT ?role ?context ?start ?end
    WHERE {
        :sergio-mattarella tvc:hasValue ?value .
        
        ?value a undo:ValueInTimeAndContext ; 
            tvc:withValue ?role ;
            tvc:withinContext ?context ;
            tvc:atTime ?time .
        
        ?time a undo:Interval ;
            ti:hasIntervalStartDate ?start .
         
        OPTIONAL {
            ?time ti:hasIntervalEndDate ?end
        }
        
        ?role a allot:Role .
    }



#### Question 7

How many times an agent has been assigned to a specific role?

    SELECT DISTINCT ?agent ?role ?context (count(?agent) AS ?count)
    WHERE {
        ?agent a undo:Agent ;
            tvc:hasValue ?value .
        
        ?value a undo:ValueInTimeAndContext ; 
            tvc:withValue ?role ;
            tvc:withinContext ?context .
        
        ?role a allot:Role .
    }
    GROUP BY ?agent ?role ?context


#### Question 8

Which roles are involved in particular contexts?

    SELECT DISTINCT ?context ?role
    WHERE {
        ?value a undo:ValueInTimeAndContext ;
            tvc:withValue ?role ;
            tvc:withinContext ?context .
            
        ?role a allot:Role .
    }
    

#### Question 9

What are all the statuses that have been associated to all the documents?

    SELECT DISTINCT ?document ?status ?start ?end
    WHERE {
        ?document a undo:Document ;
            tvc:hasValue ?value .
        
        ?value a undo:ValueInTimeAndContext ;
            tvc:withValue ?status ;
            tvc:atTime ?time .
        
        ?time a undo:Interval ;
            ti:hasIntervalStartDate ?start .
        
        OPTIONAL {
            ?time ti:hasIntervalEndDate ?end
        }
            
        ?status a undo:Status .
    }



#### Question 10

In which step of all the workflows the first version of a document has been produced?

    SELECT ?doc ?step 
    WHERE {
        ?step a undo:Step ;
            pwo:produces ?doc .
            ?doc a undo:DocumentVersion .
        FILTER NOT EXISTS {
            ?another_step a undo:Step ;
                pwo:produces ?prev_version .
            ?prev_version frbr:revision+ ?doc
        }
    }


#### Question 11

How many steps (on average) are used in each workflow?

    SELECT (avg(?n_step) as ?average)
    WHERE {
        {
            SELECT ?workflow (count(?step) as ?n_step)
            {
                ?workflow a undo:Workflow ;
                    pwo:hasStep ?step .
            } GROUP BY ?workflow
        }
    } GROUP BY ?workflow


#### Question 12

How much did it take to executing each step in each workflow execution?
    
    SELECT ?execution ?step (round(?end - ?start) as ?minutes)
    WHERE {
        {
            SELECT ?execution ?step (min(?s_date) as ?start) (max(?e_date) as ?end) {
                ?execution a undo:WorkflowExecution ;
                    pwo:involvesAction ?action .
                ?action a undo:Action ;
                    taskex:executesTask ?step ;
                    pwo:happened ?time .
                ?time a undo:Interval ;
                    ti:hasIntervalStartDate ?s_date ;
                    ti:hasIntervalEndDate ?e_date .
            } GROUP BY ?execution ?step
        }
    }


#### Question 13

What was the last entities produced by all the workflow executions?

    SELECT ?execution ?entity {
        ?execution a undo:WorkflowExecution ;
            pwo:involvesAction/taskex:executesTask ?step .
        ?step a undo:Step ;
            pwo:produces ?entity .
        FILTER NOT EXISTS {
            ?step pwo:hasNextStep ?another_step .
        }
    }"""@en ;
    dc:rights "This work is distributed under a Creative Commons Attribution License (http://creativecommons.org/licenses/by/4.0/)."@en ;
    dc:title "The United Nations System Document Ontology (UNDO)"@en ;
    ns1:preferredNamespacePrefix "undo" ;
    ns1:preferredNamespaceUri "https://w3id.org/un/ontology/undo/" ;
    rdfs:comment "The United Nations System Document Ontology (UNDO) is an OWL 2 DL ontology that aims at providing a framework for the description of all entities and the relations that are explicitly or implicitly introduced within United Nations documents (normative documents, legal documents, etc.)."@en ;
    owl:imports <http://purl.org/spar/frbr>,
        <http://purl.org/spar/pwo>,
        <http://www.essepuntato.it/2012/04/tvc>,
        <http://www.ontologydesignpatterns.org/cp/owl/timeinterval.owl>,
        oa:,
        <https://w3id.org/akn/ontology/allot/2017-04-21> ;
    owl:priorVersion <https://w3id.org/un/ontology/undo/2017-04-21> ;
    owl:versionIRI <https://w3id.org/un/ontology/undo/2017-06-01> ;
    owl:versionInfo "June 1, 2017"@en .

